renaming files

thys/examples/code/qs_quicksort.ll
@@ -94,11 +94,11 @@ define void @qs_quicksort(i64* %A, i64 %lo, i64 %hi) #0 {
   start:
     %x = insertvalue { i64, i64 } zeroinitializer, i64 %lo, 0
     %xa = insertvalue { i64, i64 } %x, i64 %hi, 1
-    call void @LLVM_Examples_qs_quicksort_f_013440878 (i64* %A, { i64, i64 } %xa)
+    call void @LLVM_Examples_qs_quicksort_f_013752572 (i64* %A, { i64, i64 } %xa)
     ret void
 }
 
-define void @LLVM_Examples_qs_quicksort_f_013440878(i64* %A, { i64, i64 } %x) #0 {
+define void @LLVM_Examples_qs_quicksort_f_013752572(i64* %A, { i64, i64 } %x) #0 {
 
   start:
     %lo = extractvalue { i64, i64 } %x, 0
@@ -111,11 +111,11 @@ define void @LLVM_Examples_qs_quicksort_f_013440878(i64* %A, { i64, i64 } %x) #0
     %tmpa = sub i64 %p, 1
     %xf = insertvalue { i64, i64 } zeroinitializer, i64 %lo, 0
     %xg = insertvalue { i64, i64 } %xf, i64 %tmpa, 1
-    call void @LLVM_Examples_qs_quicksort_f_013440878 (i64* %A, { i64, i64 } %xg)
+    call void @LLVM_Examples_qs_quicksort_f_013752572 (i64* %A, { i64, i64 } %xg)
     %tmpaa = add i64 %p, 1
     %xi = insertvalue { i64, i64 } zeroinitializer, i64 %tmpaa, 0
     %x1 = insertvalue { i64, i64 } %xi, i64 %hi, 1
-    call void @LLVM_Examples_qs_quicksort_f_013440878 (i64* %A, { i64, i64 } %x1)
+    call void @LLVM_Examples_qs_quicksort_f_013752572 (i64* %A, { i64, i64 } %x1)
     br label %ctd_if
 
   else:
